Fix bounds on wire_digits
As per
https://github.com/mit-plv/fiat-crypto/pull/86#issuecomment-255839706

src/Specific/GF25519BoundedCommon.v
@@ -59,12 +59,31 @@ Definition Build_bounded_word {lower upper} (proj_word : word64) (word_bounded :
         | false => fun x => x
         end word_bounded).
 Local Notation word_of exp := (bounded_word (fst (b_of exp)) (snd (b_of exp))).
+Local Notation unbounded_word := (bounded_word 0 (2^32-1)%Z).
+Lemma word32_to_unbounded_helper {x e : nat} : (x < pow2 e)%nat -> (Z.of_nat e <= 64)%Z -> ((0 <=? word64ToZ (ZToWord64 (Z.of_nat x))) && (word64ToZ (ZToWord64 (Z.of_nat x)) <=? 2 ^ (Z.of_nat e) - 1))%bool = true.
+Proof.
+  rewrite pow2_id; intro H; apply Nat2Z.inj_lt in H; revert H.
+  rewrite Z.pow_Zpow; simpl Z.of_nat.
+  intros H H'.
+  assert (2^Z.of_nat e <= 2^64) by auto with zarith.
+  rewrite !ZToWord64ToZ by omega.
+  match goal with
+  | [ |- context[andb ?x ?y] ]
+    => destruct x eqn:?, y eqn:?; try reflexivity; Z.ltb_to_lt
+  end;
+    intros; omega.
+Qed.
+Definition word32_to_unbounded_word (x : word 32) : unbounded_word.
+Proof.
+  refine (Build_bounded_word (Z.of_N (wordToN x)) _).
+  abstract (rewrite wordToN_nat, nat_N_Z; apply (word32_to_unbounded_helper (wordToNat_bound x)); simpl; omega).
+Qed.
 Definition bounds : list (Z * Z)
   := Eval compute in
       [b_of 25; b_of 26; b_of 25; b_of 26; b_of 25; b_of 26; b_of 25; b_of 26; b_of 25; b_of 26].
 Definition wire_digit_bounds : list (Z * Z)
   := Eval compute in
-      [b_of 25; b_of 26; b_of 25; b_of 26; b_of 25; b_of 26; b_of 25; b_of 26].
+      List.repeat (0, 2^32-1)%Z 8.
 
 Definition fe25519W := Eval cbv -[word64] in (tuple word64 (length limb_widths)).
 Definition wire_digitsW := Eval cbv -[word64] in (tuple word64 8).
@@ -85,8 +104,8 @@ Definition fe25519 :=
     let sanity := eq_refl : length bounds = length limb_widths in
     (word_of 25 * word_of 26 * word_of 25 * word_of 26 * word_of 25 * word_of 26 * word_of 25 * word_of 26 * word_of 25 * word_of 26)%type.
 Definition wire_digits :=
-  Eval cbv [fst snd] in
-    (word_of 25 * word_of 26 * word_of 25 * word_of 26 * word_of 25 * word_of 26 * word_of 25 * word_of 26)%type.
+  Eval cbv [fst snd Tuple.tuple Tuple.tuple'] in
+    Tuple.tuple unbounded_word 8.
 Definition proj1_fe25519W (x : fe25519) : fe25519W
   := let '(x0, x1, x2, x3, x4, x5, x6, x7, x8, x9) := x in
      (proj_word x0, proj_word x1, proj_word x2, proj_word x3, proj_word x4,
